FGL: make identity congruences more general

books/centaur/fgl/congruence-rules.lisp
@@ -60,6 +60,8 @@
    (arity natp :rule-classes :type-prescription))
   :layout :list)
 
+(fty::deflist fgl-id-congruence-rulelist :elt-type fgl-id-congruence-rule :true-listp t)
+
 
 
 ;; (define fgl-ev-congruence-rulelist-correct-p ((x congruence-rulelist-p))
@@ -105,49 +107,172 @@
 (fty::defmap congruence-rule-table :key-type pseudo-fnsym :val-type congruence-rulelist
   :true-listp t)
 
-(fty::defmap id-congruence-rule-table :key-type pseudo-fnsym :val-type fgl-id-congruence-rule :true-listp t)
+(fty::defmap id-congruence-rule-table :key-type pseudo-fnsym :val-type fgl-id-congruence-rulelist :true-listp t)
 
+;; ID congruences -- We want a (first-order) condition that implies the (second-order)
+;; following property: for any equivalence relation equiv, (equiv x y) => (equiv (foo z x) (foo z y))
+;; (generalized to any arity and argument position).
+;; A sufficient condition (proof below) implying this is (for all z, x, y):
+;; (or (equal (foo z x) (foo z y))
+;;     (equal (foo z x) x)).
+;; In many cases we have (equal (foo z x) x) unconditionally, which we recognize separately
+;; for convenience.
 
-(define parse-id-congruence-rule ((x pseudo-termp))
-  :returns (rule (iff (fgl-id-congruence-rule-p rule) rule))
-  :prepwork ((local (in-theory (disable cmr::pseudo-term-var-list->names-when-pseudo-term-listp)))
-             (local (defthm symbol-listp-when-pseudo-var-list-p
-                      (implies (pseudo-var-list-p x)
-                               (symbol-listp x))))
-             (local (defthm consp-assoc-equal-when-key
+;; Proof: assuming (equiv x y) and not (equiv (foo z x) (foo z y)), we have
+;; (not (equal (foo z x) (foo z y))), therefore (equal (foo z x) x) and (equal
+;; (foo z y) y).  Then (not (equiv (foo z x) (foo z y))) reduces to (not (equiv
+;; x y)), contradicting our assumption.
+(local (in-theory (disable cmr::pseudo-term-var-list->names-when-pseudo-term-listp)))
+(local (defthm symbol-listp-when-pseudo-var-list-p
+         (implies (pseudo-var-list-p x)
+                  (symbol-listp x))))
+
+(local (defthm pseudo-termp-nth
+         (implies (pseudo-term-listp x)
+                  (pseudo-termp (nth n x)))
+         :hints(("Goal" :in-theory (enable pseudo-term-listp nth)))))
+
+(local (defthm pseudo-term-var-nth
+         (implies (and (cmr::pseudo-term-var-listp x)
+                       (< (nfix n) (len x)))
+                  (pseudo-term-case (nth n x) :var))
+         :hints(("Goal" :in-theory (enable cmr::pseudo-term-var-listp len nth)))))
+
+;; This recognizes (equal (foo z x) x) (generalized by arity/position), and
+;; returns the rule (containing function, arity, position).
+(define parse-simple-id-congruence ((x pseudo-termp))
+  :returns (mv (rule (iff (fgl-id-congruence-rule-p rule) rule))
+               (vars pseudo-term-listp))
+  :prepwork ((local (defthm consp-assoc-equal-when-key
                       (implies k
                                (iff (consp (Assoc-equal k x)) (assoc-equal k x))))))
   (pseudo-term-case x
-    :fncall (and (eq x.fn 'equal)
-                 (eql (len x.args) 2)
-                 (b* ((arg2 (second x.args))
-                      (arg2-var
-                       (pseudo-term-case arg2
-                         :var arg2.name
-                         :lambda
-                         (pseudo-term-case arg2.body
-                           :var (and (equal arg2.body
-                                            (cdr (assoc arg2.body.name
-                                                        (pairlis$ arg2.formals
-                                                                  arg2.args))))
-                                     arg2.body.name)
-                           :otherwise nil)
-                         :otherwise nil))
-                      ((unless arg2-var) nil)
-                   ;; (let ((arg2 (second x.args)))
-                   ;;   (pseudo-term-case 
-                   ;;   (or (pseudo-term-case (second x.args) :var)
-                   ;;     (pseudo-term-case (second x.args) :var)
-                      (arg1 (first x.args)))
-                   (pseudo-term-case arg1
-                     :fncall (and (cmr::pseudo-term-var-listp arg1.args)
-                                  (b* ((vars (cmr::pseudo-term-var-list->names arg1.args)))
-                                    (and (no-duplicatesp-eq vars)
-                                         (b* ((idx (acl2::index-of arg2-var vars)))
-                                           (and idx
-                                                (fgl-id-congruence-rule arg1.fn idx (len vars)))))))
-                     :otherwise nil)))
-    :otherwise nil))
+    :fncall (if (and (eq x.fn 'equal)
+                     (eql (len x.args) 2))
+                (b* ((arg2 (second x.args))
+                     (arg2-var
+                      (pseudo-term-case arg2
+                        :var arg2.name
+                        :lambda
+                        (pseudo-term-case arg2.body
+                          :var (and (equal arg2.body
+                                           (cdr (assoc arg2.body.name
+                                                       (pairlis$ arg2.formals
+                                                                 arg2.args))))
+                                    arg2.body.name)
+                          :otherwise nil)
+                        :otherwise nil))
+                     ((unless arg2-var) (mv nil nil))
+                     ;; (let ((arg2 (second x.args)))
+                     ;;   (pseudo-term-case 
+                     ;;   (or (pseudo-term-case (second x.args) :var)
+                     ;;     (pseudo-term-case (second x.args) :var)
+                     (arg1 (first x.args)))
+                  (pseudo-term-case arg1
+                    :fncall (b* (((unless (cmr::pseudo-term-var-listp arg1.args)) (mv nil nil))
+                                 (vars (cmr::pseudo-term-var-list->names arg1.args))
+                                 ((unless (no-duplicatesp-eq vars)) (mv nil nil))
+                                 (idx (acl2::index-of arg2-var vars))
+                                 ((unless idx) (mv nil nil)))
+                              (mv (fgl-id-congruence-rule arg1.fn idx (len vars)) arg1.args))
+                    :otherwise (mv nil nil)))
+              (mv nil nil))
+    :otherwise (mv nil nil))
+  ///
+  (defret pseudo-term-var-listp-of-<fn>
+    (cmr::pseudo-term-var-listp vars)))
+
+
+(define parse-simple-disjunction ((x pseudo-termp))
+  :returns (mv ok (left pseudo-termp) (right pseudo-termp))
+  (pseudo-term-case x
+    :fncall (case x.fn
+              (if
+                  (if (or (equal (first x.args)
+                                 (second x.args))
+                          (equal (second x.args) ''t))
+                      (mv t (first x.args) (third x.args))
+                    (mv nil nil nil)))
+              (implies
+               (let ((arg1 (first x.args)))
+                 (pseudo-term-case arg1
+                   :fncall (if (eq arg1.fn 'not)
+                               (mv t (first arg1.args) (second x.args))
+                             (mv nil nil nil))
+                   :otherwise (mv nil nil nil))))
+              (t (mv nil nil nil)))
+    :otherwise (mv nil nil nil)))
+
+(define parse-id-congruence-equivalence ((rule fgl-id-congruence-rule-p)
+                                         (vars pseudo-term-listp)
+                                         (x pseudo-termp))
+  :guard (cmr::pseudo-term-var-listp vars)
+  :returns (diff-var pseudo-termp)
+  (b* (((fgl-id-congruence-rule rule)))
+    (pseudo-term-case x
+      :fncall (and (eq x.fn 'equal)
+                   (b* (((list arg1 arg2) x.args)
+                        ((unless (and (pseudo-term-case arg1 :fncall)
+                                      (pseudo-term-case arg2 :fncall)))
+                         nil)
+                        ((pseudo-term-fncall arg1))
+                        ((pseudo-term-fncall arg2))
+                        ((unless (and (eq arg1.fn rule.fn)
+                                      (eq arg2.fn rule.fn)))
+                         nil)
+                        (vars (pseudo-term-list-fix vars))
+                        (diff-args (cond ((mbe :logic (pseudo-term-list-equiv arg1.args vars)
+                                               :exec (equal arg1.args vars))
+                                          arg2.args)
+                                         ((mbe :logic (pseudo-term-list-equiv arg2.args vars)
+                                               :exec (equal arg2.args vars))
+                                          arg1.args))))
+                     (and diff-args
+                          (cmr::pseudo-term-var-listp diff-args)
+                          (no-duplicatesp-eq (cmr::pseudo-term-var-list->names diff-args))
+                          (b* ((diff-var (nth rule.id-index diff-args)))
+                            (and (not (member-equal diff-var vars))
+                                 (equal (update-nth rule.id-index (nth rule.id-index diff-args) vars)
+                                        diff-args)
+                                 ;; (fgl-id-congruence-rule-fix rule)
+                                 diff-var)))))
+      :otherwise nil))
+  ///
+  (local (defthm len-of-update-nth
+           (equal (len (update-nth n v y))
+                  (max (len y) (+ 1 (nfix n))))
+           :hints(("Goal" :in-theory (enable len update-nth)))))
+  (local (defthm len-of-update-nth-free
+           (implies (equal x (update-nth n v y))
+                    (equal (len x)
+                           (max (len y) (+ 1 (nfix n)))))))
+  (local (defthm max-when-less
+           (implies (and (< x y)
+                         (integerp x) (integerp y))
+                    (equal (max y (+ 1 x)) y))))
+  (local (in-theory (disable max)))
+  (defret pseudo-term-kind-of-<fn>
+    (b* (((fgl-id-congruence-rule rule)))
+      (implies (and diff-var
+                    (equal (len vars) rule.arity)
+                    (< rule.id-index rule.arity))
+               (pseudo-term-case diff-var :var)))))
+
+(define parse-id-congruence-rule ((x pseudo-termp))
+  :returns (rule (iff (fgl-id-congruence-rule-p rule) rule))
+  (b* (((mv rule ?vars) (parse-simple-id-congruence x))
+       ((when rule) rule)
+       ((mv ok left right) (parse-simple-disjunction x))
+       ((unless ok) nil)
+       ((mv rule vars other-term)
+        (b* (((mv rule vars) (parse-simple-id-congruence left))
+             ((when rule) (mv rule vars right))
+             ((mv rule vars) (parse-simple-id-congruence right)))
+          (mv rule vars left)))
+       ((unless rule) nil)
+       (diff-var
+        (parse-id-congruence-equivalence rule vars other-term)))
+    (and diff-var rule)))
 
 (define check-id-congruence-rune ((rune fgl-id-congruence-rune-p)
                                   (w plist-worldp))
@@ -170,7 +295,7 @@
        ((mv errmsg rest) (id-congruence-table-from-runes (cdr runes) w))
        ((when errmsg) (mv errmsg nil))
        ((fgl-id-congruence-rule rule)))
-    (mv nil (hons-acons rule.fn rule rest))))
+    (mv nil (hons-acons rule.fn (cons rule (cdr (hons-get rule.fn rest))) rest))))
        
 
 
@@ -208,8 +333,31 @@
             (table fgl-id-congruence-rules 'fgl-id-congruence-rules
                    (cons ',rune (fgl-id-congruence-runes world))))))
 
+(defmacro def-fgl-id-congruence (name call index &rest kwd-args)
+  (b* (((unless (and (symbolp name)
+                     (symbol-listp call)
+                     (consp call)
+                     (no-duplicatesp-eq (cdr call))
+                     (posp index)
+                     (< index (len call))))
+        (er hard? 'def-fgl-id-congruence "Malformed args"))
+       (arg (nth index call))
+       (alt-arg (intern-in-package-of-symbol
+                 (concatenate 'string (symbol-name arg) "-EQUIV") (car call))))
+    `(progn (defthm ,name
+              (or (equal ,call ,arg)
+                  (equal ,call ,(update-nth index alt-arg call)))
+              :rule-classes nil
+              . ,kwd-args)
+            (add-fgl-id-congruence ,name))))
+
 (local (defun foo (x) x))
+(local (define bar (x) x))
 (local (add-fgl-id-congruence foo))
+(local (add-fgl-id-congruence bar))
+(local (defun baz (x y z) (if x y z)))
+(local (def-fgl-id-congruence baz-id-cong-1 (baz x y z) 2))
+(local (def-fgl-id-congruence baz-id-cong-2 (baz x y z) 3))
 
 
 (defxdoc add-fgl-congruence
@@ -225,18 +373,224 @@ consumed by FGL.</p>
 <p>See also @(see add-fgl-id-congruence) for an additional kind of rule
 appropriate to identity functions.</p>")
 
+
+
+(defsection conditional-identity-implies-congruence-propagation
+  :parents (add-fgl-id-congruence)
+  :short "Proof that the conditional identity property implies the congruence propagation property"
+  :long "<p>See @(see add-fgl-id-congruence) for details.</p>
+<p>Events:</p>
+@(`*conditional-identity-implies-congruence-propagation-events*`)"
+  (defconst *conditional-identity-implies-congruence-propagation-events*
+   '(progn
+      (encapsulate
+        (((f * *) => *))
+
+        (local (defun f (p x)
+                 (declare (ignore p))
+                 x))
+        (defthm conditional-identity
+          (or (equal (f p x) (f p y))
+              (equal (f p x) x))
+          :rule-classes nil))
+
+      (encapsulate
+        (((eqv * *) => *))
+
+        (local (defun eqv (x y) (equal x y)))
+        (defequiv eqv))
+
+      (defthm congruence-propagation
+        (implies (eqv x y)
+                 (eqv (f p x) (f p y)))
+        :hints (("goal" :use ((:instance conditional-identity (y x) (x y))
+                              (:instance conditional-identity))))
+        :rule-classes nil)))
+  (local (make-event *conditional-identity-implies-congruence-propagation-events*)))
+
+
+(defsection congruence-propagation-implies-conditional-identity
+  :parents (add-fgl-id-congruence)
+  :short "Proof that the congruence propagation property implies the conditional identity property"
+  :long "<p>See @(see add-fgl-id-congruence) for details.</p>
+<p>Events:</p>
+@(`*congruence-propagation-implies-conditional-identity-events*`)"
+  (defconst *congruence-propagation-implies-conditional-identity-events*
+    '(progn
+       (encapsulate
+         (((f * *) => *)
+          ((x) => *)
+          ((y) => *)
+          ((p) => *))
+
+         (local (defun f (p x)
+                  (declare (ignore p))
+                  (not x)))
+         (local (defun x () t))
+         (local (defun y () nil))
+         (local (defun p () nil))
+         (defthm not-conditional-identity
+           (not (or (equal (f (p) (x)) (f (p) (y)))
+                    (equal (f (p) (x)) (x))))
+           :rule-classes nil))
+
+       (defun z ()
+         (car (set-difference-equal '(0 1 2) (list (x) (y)))))
+
+       (defthm z-not-x
+         (not (equal (z) (x))))
+
+       (defthm z-not-y
+         (not (equal (z) (y))))
+
+       (in-theory (disable z (z)))
+
+       (defun eqv (a b)
+         (let ((s (cond ((not (equal (f (p) (x)) (y)))
+                         (list (x) (y) (f (p) (y))))
+                        ((not (equal (f (p) (y)) (x)))
+                         (list (x) (y)))
+                        ((equal (f (p) (z)) (x))
+                         (list (x) (z)))
+                        (t (list (y) (z) (f (p) (z)))))))
+           (iff (member a s) (member b s))))
+
+       (defun a ()
+         (cond ((not (equal (f (p) (x)) (y))) (x))
+               ((not (equal (f (p) (y)) (x))) (x))
+               ((equal (f (p) (z)) (x)) (x))
+               (t (y))))
+
+       (defun b ()
+         (cond ((not (equal (f (p) (x)) (y))) (y))
+               ((not (equal (f (p) (y)) (x))) (y))
+               ((equal (f (p) (z)) (x)) (z))
+               (t (z))))
+
+       (defthm not-congruent
+         (not (implies (eqv (a) (b))
+                       (eqv (f (p) (a)) (f (p) (b)))))
+         :hints (("goal" :use not-conditional-identity)))
+
+       (defequiv eqv)))
+  (local (make-event *congruence-propagation-implies-conditional-identity-events*)))
+     
+
+
+
+
+
 (defxdoc add-fgl-id-congruence
   :parents (fgl-rewrite-rules)
   :short "Add an identity congruence rule to FGL's theory"
-  :long "<p>It is sometimes convenient to use identity functions to mark terms in the
-FGL rewriter. A special property of these is that if we are rewriting the call
-of an identity function in some equivalence context, it is sound to rewrite the
-argument of the identity function in the same equivalence context. This
-behavior can't be replicated with regular congruence rules except by proving
-such a rule for every equivalence context.</p>
+  :long "<h3>Usage:</h3>
+@({
+ (add-fgl-id-congruence thmname)
+ })
+<p>where @('thmname') is the name of a theorem of either of the following forms:
+@({
+ (equal (f x1 ... xi ... xn) xi)
+ })
+or
+@({
+ (or (equal (f x1 ... xi ... xn) (f x1 ... yi ... xn))
+     (equal (f x1 ... xi ... xn) xi))
+ })
+where @('f') is some function and @('yi') occurs in the argument list of its
+call of @('f') in the same position as argument @('xi') occurs in other
+calls. The form of this theorem is justified in the Theory section below.</p>
 
-<p>This macro takes a single argument which is the name of a formula of the
-form @('(equal (<fn> <var>) <var>)'). Notably, for a function defined using
-@('(defun fn (x) x)'), the function's name itself has such a formula. Calling
-this macro with such an argument lets FGL use the equivalence context of the
-call of fn when rewriting the argument of fn.</p> ")
+<p>See also @('def-fgl-id-congruence'), which additionally generates and
+attempts to prove the required theorem.</p>
+
+<h3>Function</h3>
+<p>When such a theorem is added to FGL's theory, it allows rewriting of the
+@('xi') argument position under an equivalence relation whenever we are
+rewriting the outer call of @('f') under that equivalence relation. In effect,
+it is as if we added the following congruence rule (see @(see
+acl2::congruence)) for all equivalences @('eqv'):</p>
+@({
+ (implies (eqv xi yi)
+          (eqv (f x1 ... xi ... xn) (f x1 ... yi ... xn)))
+ })
+
+<h3>Theory</h3>
+<p>An identity function @('(f x) = x') has the property that for any
+equivalence relation @('eqv'),
+@({
+ (implies (eqv x y)
+          (eqv (f x) (f y))),
+ })
+that is, if we are rewriting a call of @('f') under some equivalence context,
+we can rewrite its argument under that same context. (Call this the
+congruence propagation property for argument 1 of @('f').)</p>
+
+<p>This isn't only true of identity functions. For example, if @('(g x y z)')
+equals @('(if x y z)'), then g has this property for both its second and third
+argument, i.e. for any equivalence @('eqv'),
+@({
+ (implies (eqv y y-equiv)
+          (eqv (g x y z) (g x y-equiv z)))
+})
+and
+@({
+ (implies (eqv z z-equiv)
+          (eqv (g x y z) (g x y z-equiv))), }) that is, if rewriting a call of
+ @('g') under some equivalence context, we can rewrite both its second and
+ third arguments under that equivalence context.</p>
+
+<p>The first-orderness of ACL2 prevents us from straightforwardly expressing
+this property in terms of \"for any equivalence relation\". However, the
+following property (call it the conditional identity property) is equivalent to
+the congruence propagation property:</p>
+@({
+ (or (equal (f x) (f y))
+     (equal (f x) x))
+ })
+<p>The proof is in two parts, in sections @(see conditional-identity-implies-congruence-propagation)
+and @(see congruence-propagation-implies-conditional-identity). We outline how the proofs work in broad strokes.</p>
+
+<p>In @(see conditional-identity-implies-congruence-propagation)
+ a function @('f') is introduced with the sole constraint that it satisfies the conditional identity property on its second argument, then another function @('eqv') is introduced with the sole constraint that it is an equivalence relation. Given these two assumptions, we then show that @('f') satisfies the congruence propagation property with respect to @('eqv').</p>
+
+<p>We take a slightly more roundabout tactic in @(see
+congruence-propagation-implies-conditional-identity) in order to avoid stating
+the assumption that @('f') satisfies the congruence propagation property for
+all possible equivalence relations. Instead, we introduce @('f') with the
+constraint that it does not satisfy the congruence propagation property; that
+is, for certain arguments (0-ary functions constrained along with @('f')), that
+property is untrue. We then define a function @('eqv') in terms of @('f') and
+those arguments, showing that it is an equivalence relation and that there are
+arguments to @('f') for which the congruence propagation property with respect
+to @('eqv') is then violated.</p>")
+
+
+(defxdoc def-fgl-id-congruence
+  :parents (fgl-rewrite-rules)
+  :short "Prove and add an identity congruence rule to FGL's theory"
+  :long "<p>See @(see add-fgl-id-congruence) for an explanation of identity congruence rules.</p>
+
+<p>Usage:
+@({
+ (def-fgl-id-congruence thmname (f x1 ... xn) index
+   :hints hints)
+ })
+where @('thmname') is the name of the theorem to be generated, @('f') is some
+function, @('x1 ... xn') a duplicate-free list of variables, and @('index') is
+the (1-based) index of the identity argument (a positive integer less than or
+equal to the arity of @('f'). (The index is 1-based for compatibility with
+@(see acl2::defcong).)</p>
+
+<p>This generates a theorem of the following form
+@({
+ (defthm thmname
+   (or (equal (f x1 ... xi ... xn) xi)
+       (equal (f x1 ... xi ... xn) (f x1 ... xi-equiv ... xn)))
+  :hints hints
+  :rule-classes nil)
+ })
+
+where @('xi') is the variable in position @('index') of the provided argument
+list. After the theorem is admitted the theorem is registered as an identity
+congruence for FGL using @(see add-fgl-id-congruence).</p>")
+
